More efficient contract join

hol/symb_exec/p4_symb_execScript.sml
@@ -1,6 +1,8 @@
 open HolKernel boolLib liteLib simpLib Parse bossLib;
 
-open p4Theory;
+open p4Theory listTheory;
+
+open symb_execTheory;
 
 val _ = new_theory "p4_symb_exec";
 
@@ -17,6 +19,32 @@ Definition p4_contract_def:
   (P ==> ?n. arch_multi_exec ctx s n <> NONE /\ !s'. arch_multi_exec ctx s n = SOME s' ==> Q s')
 End
 
+(* TODO: This can be written using FOLDL *)
+Definition p4_contract_list_def:
+ (p4_contract_list P (h::[]) ctx s Q = p4_contract (P ==> h) ctx s Q) /\
+ (p4_contract_list P (h::t) ctx s Q = (p4_contract (P ==> h) ctx s Q /\ p4_contract_list P t ctx s Q)) /\
+ (p4_contract_list P [] ctx s Q = T)
+End
+
+Theorem p4_contract_list_REWR:
+ !R P P_list ctx s Q b.
+ (((p4_contract (R ==> P) ctx s Q /\ b) /\ p4_contract_list R P_list ctx s Q) <=> (b /\ p4_contract_list R (P::P_list) ctx s Q)) /\
+ ((p4_contract (R ==> P) ctx s Q /\ p4_contract_list R P_list ctx s Q) <=> p4_contract_list R (P::P_list) ctx s Q) /\
+ ((p4_contract (R ==> P) ctx s Q /\ b) <=> (b /\ p4_contract_list R [P] ctx s Q))
+Proof
+Cases_on ‘P_list’ >> (
+ fs[p4_contract_list_def] >>
+ metis_tac[]
+)
+QED
+
+Theorem p4_contract_imp_REWR:
+ !P ctx s Q.
+ ((p4_contract P ctx s Q) <=> (p4_contract (T ==> P) ctx s Q))
+Proof
+fs[p4_contract_def]
+QED
+
 Theorem p4_symb_exec_to_contract:
 !P ctx s n s' Q.
 (P ==> arch_multi_exec ctx s n = SOME s' /\ Q s') ==>
@@ -30,6 +58,8 @@ rpt strip_tac >> (
 )
 QED
 
+(* For branching and unification *)
+
 Theorem p4_symb_exec_unify:
 !P1 P2 ctx s Q.
 p4_contract (P1 /\ P2) ctx s Q ==>
@@ -40,28 +70,25 @@ fs[p4_contract_def] >>
 metis_tac []
 QED
 
-(* For branching and unification *)
-
-(* OLD, with superfluous base case
-Definition list_disj_def:
- (list_disj [] = T) /\
- (list_disj (h::t) = (h \/ list_disj t))
-End
-*)
-(* TODO: What should the base case be? *)
-Definition list_disj_def:
- (list_disj (h::t) =
-  if t = []
-  then h
-  else (h \/ list_disj t))
-End
-
-Definition p4_contract_list_def:
- (p4_contract_list [] P ctx s Q = p4_contract P ctx s Q) /\
- (p4_contract_list (h::t) P ctx s Q =
-  if t = []
-  then p4_contract (h /\ P) ctx s Q
-  else (p4_contract (h /\ P) ctx s Q /\ p4_contract_list t P ctx s Q))
-End
+(* Note that the point with this theorem is to explicitly
+ * incorporate R ==> disj_list P_list ("disj_thm") as a premise,
+ * so you don't need to rewrite or reason using
+ * it when obtaining the conclusion *)
+Theorem p4_symb_exec_unify_n_gen:
+!P_list R P' ctx s Q.
+(R ==> disj_list P_list) ==>
+p4_contract_list R P_list ctx s Q ==>
+p4_contract R ctx s Q
+Proof
+Induct_on ‘P_list’ >> (
+ fs [disj_list_def, p4_contract_list_def, p4_contract_def]
+) >>
+rpt strip_tac >>
+Cases_on ‘P_list’ >> (
+ fs [disj_list_def, p4_contract_list_def, p4_contract_def]
+) >>
+rpt strip_tac >>
+fs[]
+QED
 
 val _ = export_theory ();
